Added conversion from NFA to DFA
- Added new file ToNFA
- Changed definition of delta_star for both NFA and DFA
- Corrected a definition for dfa_delta_to_nfa_delta

lean4/Automaton/DFA/Basic.lean
@@ -3,47 +3,87 @@ import Automaton.Language.Basic
 /-!
   This file contains the definition of a DFA as well as a few fundamental operations it can do
   * `δ_star` and `accepts` functions.
-  
-  * Also asserts the decidability of the language of DFA
+  * Asserts the decidability of the language of DFA
+  * Provides a definition for equality of DFA and proves basic properties about the equality
+    * Two DFAs are equal, if they accept the same language
 -/
 
 namespace DFA
 
-structure DFA where
+structure DFA (σ : Type _) where
   q : Type _    -- states
   init : q      -- initial state
   fs : Set q    -- accepting states
-  σ : Type _    -- alphabet
   δ : q → σ → q -- transition function
   [d : DecidablePred fs]
 
-variable (t : DFA)
+variable {σ : Type _ } (α : DFA σ) (r s t : DFA σ)
 
 -- δ* function
 -- the state reached after following all transitions given a word
--- args : dfa , word , initial state 
--- (could be defined without init but words would then be reversed as written, see Examples)
-def δ_star : (w : word t.σ) → (initState : t.q) → t.q
-  | [] , cur => cur
-  | e :: es , cur => δ_star es (t.δ cur e)
+-- the first letter in list is the last character consumed
+def δ_star : (w : word σ) → t.q
+  | [] => t.init
+  | e :: es => t.δ (δ_star es) e 
 
 -- whether a DFA accepts a word
-def accepts : (w : word t.σ) → Prop := by
+def dfa_accepts : (w : word σ) → Prop := by
   intro w
-  have f := δ_star t w t.init
+  have f := δ_star t w
   apply f ∈ t.fs
 
-def dfaLang : Lang t.σ := fun w => accepts t w
+def dfaLang : Lang σ := fun w => dfa_accepts t w
 
 -- DFA language is decidable
-instance decidableLang (w : word t.σ) [d : DecidablePred (t.fs)] : Decidable (accepts t w) := by
-  dsimp [accepts]
+instance decidableLang (w : word σ) [d : DecidablePred (t.fs)] : Decidable (dfa_accepts t w) := by
+  dsimp [dfa_accepts]
   generalize δ_star t w = e
   apply d
 
 -- the set predicate is decidable
 instance decDFA : DecidablePred (t.fs) := by
   exact t.d
-  
+
+-- equality of DFAs
+def eq : Prop := ∀ w : word σ , dfa_accepts t w ↔ dfa_accepts s w
+
+private theorem eq.refl : eq t t := by
+  dsimp [eq]
+  intro w
+  apply Iff.intro <;> (intro ; assumption) 
+
+private theorem eq.trans : eq t s → eq s r → eq t r := by
+  intro eq₁ eq₂
+  dsimp [eq] at eq₁ eq₂
+  dsimp [eq]
+  intro w
+  apply Iff.intro
+  · intro r
+    apply (Iff.mp (eq₁ w))
+    apply (Iff.mp (eq₂ w))
+    exact r
+  · intro t
+    apply (Iff.mpr (eq₂ w))
+    apply (Iff.mpr (eq₁ w))
+    exact t
+
+private theorem eq.sym : eq t s → eq s t := by
+  intro h
+  dsimp [eq]
+  dsimp [eq] at h
+  intro w
+  apply Iff.intro <;> intro <;> (first | apply (Iff.mp (h w)) | apply (Iff.mpr (h w))) <;> assumption
+
+-- dfa accepts nil iff init is final
+theorem dfa_accepts_nil_iff_final : dfa_accepts t [] ↔ t.init ∈ t.fs := by
+  apply Iff.intro
+  · intro h
+    dsimp [dfa_accepts, δ_star ] at h
+    exact h
+  · intro e
+    dsimp [dfa_accepts]
+    exact e
+
+
 
 end DFA
