lean4/Automaton/NFA/Basic.lean
@@ -8,31 +8,41 @@ import Automaton.Language.Basic
 
 namespace NFA
 
-structure NFA where
+structure NFA (σ : Type _) where
   q : Type _        -- states
   init : q          -- initial state
   fs : Set q        -- accepting states
-  σ : Type _        -- alphabet
   δ : q → σ → Set q -- transition function
   [d : DecidablePred fs]
 
-variable (t : NFA)
+variable {σ : Type _} (t : NFA σ)
 
 -- one step in the operation of NFA, consuming one character
 -- take the union of all sets of states reachable from current set of states
-def δ_step (e : t.σ) (q : Set t.q) : Set t.q := ⋃₀ {t.δ a e | a ∈ q}
+def δ_step  (q : Set t.q) (e : σ) : Set t.q := ⋃₀ {t.δ a e | a ∈ q}
 
 -- δ* function for NFA
 -- returns set of states reached after inputting a word
-def δ_star (q : Set t.q) : (w : word t.σ) → Set t.q 
-  | [] => q
-  | e :: es => δ_star (δ_step t e q) es
+def δ_star : (w : word σ) → Set t.q 
+  | [] => {t.init}
+  | e :: es => δ_step t (δ_star es) e 
 
 -- Whether a word is in the language that the NFA accepts
-def accepts (w : word t.σ) : Prop := by
-  have δ_fs : Set t.q := δ_star t { t.init } w
+def nfa_accepts (w : word σ) : Prop := by
+  have δ_fs : Set t.q := δ_star t w
   have i := Set.inter δ_fs t.fs 
   exact i.Nonempty
 
-
+-- nfa accepts nil iff init is final
+theorem nfa_accepts_nil_iff_final : nfa_accepts t [] ↔ t.init ∈ t.fs := by
+  apply Iff.intro
+  · intro h
+    dsimp [nfa_accepts, δ_star ] at h
+    apply (Iff.mp Set.singleton_inter_nonempty)
+    exact h
+  · intro e
+    dsimp [nfa_accepts]
+    apply (Iff.mpr Set.singleton_inter_nonempty)
+    exact e
+    
 end NFA
